\begin{answer}
\begin{align*}
&\mathbb{E}_{y\sim p(y;\theta)}[-\nabla^2_{\theta'}\log p(y;\theta')|_{\theta' = \theta}] \\
= & \mathbb{E}_{y\sim p(y;\theta)}[-\nabla_{\theta'}( \frac{1}{p(y;\theta')} \nabla_{\theta'}^T p(y;\theta'))|_{\theta' = \theta} ]\\
=& \mathbb{E}_{y\sim p(y;\theta)}[-( -\frac{1}{p(y;\theta')^2}\nabla_{\theta'}p(y;\theta')\nabla^T_{\theta'}p(y;\theta')+ \frac{1}{p(y;\theta')}\nabla^2_{\theta'} p(y;\theta'))|_{\theta' = \theta} ]\\
= &\mathbb{E}_{y\sim p(y;\theta)}[\nabla_{\theta'}\log p(y;\theta')\nabla^T_{\theta'}\log p(y;\theta')|_{\theta' = \theta}]+\int_{-\infty}^{\infty}p(y;\theta)\frac{1}{p(y;\theta)}\nabla^2_{\theta'} p(y;\theta)dy\\
= &\mathcal{I}(\theta) + \nabla^2_{\theta'}\int_{-\infty}^{\infty} p(y;\theta)dy\\
= &\mathcal{I}(\theta)
\end{align*}

\end{answer}
