\begin{answer}
For convenience we set $ \nabla_{\theta'}f(\theta) $ as $ \nabla_{\theta'}f(\theta')|_{\theta' = \theta} $.

Lagrangian
\begin{align*}
 L(\theta, \lambda) = l(\theta) + d^T\nabla_{\theta'}l(\theta) - \lambda(\frac{1}{2}d^T\mathcal{I}(\theta)d - c) 
 \end{align*}
 \begin{align}
 \frac{\partial L}{\partial d} = \nabla_{\theta'}l(\theta) - \lambda\mathcal{I}(\theta)d = 0 \Rightarrow
 d = \frac{ \mathcal{I}(\theta)^{-1}\nabla_{\theta'}l(\theta)}{\lambda} \\ 
 \frac{\partial L}{\partial \lambda} = \frac{1}{2}d^T\mathcal{I}(\theta)d - c = 0
\end{align}
sub (1) into (2):
\[ \frac{\nabla_{\theta'}l(\theta)^T\mathcal{I}(\theta)^{-1}\nabla_{\theta'}l(\theta)}{2c} = \lambda^2 \]
Since we are finding an ascent direction, so $ d^T\nabla_{\theta'}l(\theta) $ should be positive, i.e.  \[ \frac{\nabla_{\theta'}l(\theta)^T\mathcal{I}(\theta)^{-1}\nabla_{\theta'}l(\theta)}{\lambda} > 0  \]
note that $ \mathcal{I}(\theta) $ is positive defined so the above formula $ \Leftrightarrow \lambda > 0 $
then
\[ \lambda = \sqrt{\frac{\nabla_{\theta'}l(\theta)^T\mathcal{I}(\theta)^{-1}\nabla_{\theta'}l(\theta)}{2c}}  \]
and 
\[ d = \sqrt{\frac{2c}{\nabla_{\theta'}l(\theta)^T\mathcal{I}(\theta)^{-1}\nabla_{\theta'}l(\theta)}}\mathcal{I}(\theta)^{-1}\nabla_{\theta'}l(\theta) \]


 \end{answer}
