\begin{answer}
    \begin{enumerate}
    	\item
    	    	Obviously,
\begin{align*}
J(\theta) =& \frac{1}{2} 	\begin{bmatrix}
\theta^Tx^{(1)}-y^{(1)}, & \cdots, & \theta^Tx^{(m)}-y^{(m)}
\end{bmatrix} \begin{bmatrix}
w^{(1)}& & \\
& \ddots &\\
& & w^{(m)}
\end{bmatrix}\begin{bmatrix}
\theta^Tx^{(1)}-y^{(1)}\\
\vdots\\
\theta^Tx^{(m)}-y^{(m)}
\end{bmatrix}\\
= &(\theta^TX^T-y^T)W(X\theta -y) \qquad \quad(\mbox{with}\  W = \frac{1}{2}
\mbox{diag}(w^{(1)},...,w^{(m)})\ )\\
= &(X\theta-y)^TW(X\theta-y)
\end{align*}
\item
\[ \frac{\partial J}{\partial \theta}=\frac{\partial }{\partial \theta}(\theta^TX^TWX\theta-2\theta^TX^TWy+y^TWy)=2X^TWX\theta-2X^TWy \]
so if we set $ w^{(i)}=2,\frac{\partial J}{\partial \theta}=0 $ then $ W=\frac{1}{2}I_{(m)}$ and $ \theta=(X^TX)^{-1}X^T{y}. $
\item
\[ p(y|X;\theta) = \prod_{i=1}^{m}p(y^{(i)}|x(^{i});\theta) = (2\pi)^{(-m/2)}(\prod_{i=1}^{m}\sigma^{(i)})^{-1}\exp\left( -\sum_{i=1}^{m}\frac{(y^{(i)}-\theta^Tx^{(i)})^2}{2(\sigma^{(i)})^2}\right)  \]
let $ w^{(i)} = \frac{1}{(\sigma^{(i)})^2}  $ and use the result in ii. to solve the regression problem.
    \end{enumerate}

\end{answer}
