\begin{answer}
since $ \int b(y)\exp(\eta y -a(\eta))dy =1$
we have
\begin{align*}
	0 = &\frac{\partial }{\partial \eta^2}\int b(y)\exp(\eta y -a(\eta))dy \\
	  = &\int \frac{\partial }{\partial \eta}\left( b(y)\exp(\eta y -a(\eta))(y-a'(\eta))\right) dy \\
	  = &\int \left( b(y)\exp(\eta y -a(\eta))(y-a'(\eta))^2-b(y)\exp(\eta y -a(\eta))a''(\eta)\right) dy\\
	  = &\int \left( b(y)\exp(\eta y -a(\eta))(y-\mathbb{E}[y;\eta])^2dy-a''(\eta)\right) \\
\end{align*}
which implies
\[ \mbox{Var}(Y;\eta)=a''(\eta) \]
\end{answer}
