\begin{answer}
By Bayes rule we have
\begin{align*}
p(y=1|x,\phi,\mu_0,\mu_1,\sigma) &= \frac{p(x|y=1)p(y=1)}{p(x|y=0)p(y=0)+p(x|y=1)p(y=1)}\\
&=\frac{1}{1+\frac{p(x|y=0)p(y=0)}{p(x|y=1)p(y=1)}}\\
&=\frac{1}{1+\exp\left(-\frac{1}{2}(\mu_{0}^T \Sigma^{-1} \mu_{0}-\mu_{1}^T \Sigma^{-1} \mu_{1})+(\mu_{0}-\mu_1)^T\Sigma^{-1}x+log\frac{1-\phi}{\phi}\right)}
\end{align*}
so we can take
$$
\theta_0 = -\frac{1}{2}(\mu_{0}^T \Sigma^{-1} \mu_{0}-\mu_{1}^T \Sigma^{-1} \mu_{1})-log\frac{1-\phi}{\phi},\theta = \Sigma^{-1}(\mu_{0}-\mu_1)
$$
\end{answer}
